implement PrepareSync

ironfleet/src/Dafny/Distributed/Protocol/ZooKeeper/LearnerHandler.dfy
@@ -9,13 +9,13 @@ import opened ZooKeeper_ZKDatabase
 import opened ZooKeeper_Environment
 
 
-datatype LearnerHandlerState = LH_HANDSHAKE_A | LH_HANDSHAKE_B | LH_DECIDE_SYNC | LH_SYNC | LH_RUNNING | LH_ERROR
+datatype LearnerHandlerState = LH_HANDSHAKE_A | LH_HANDSHAKE_B | LH_PREP_SYNC | LH_SYNC | LH_RUNNING | LH_ERROR
 datatype SyncMode = SNAP | DIFF | TRUNC
 
 /*
 * LH_HANDSHAKE_A: Receive FOLLOWERINFO, wait for quorum, then send new epoch
 * LH_HANDSHAKE_B: Wait for a quorum of ACKEPOCH response. This ends the handshake with follower
-* LH_DECIDE_SYNC: 
+* LH_PREP_SYNC: 
 */
 
 
@@ -29,6 +29,7 @@ datatype LearnerHandler = LearnerHandler(
     globals: LeaderGlobals,
 
     // Local state
+    queuedPackets: seq<ZKMessage>,
     newEpoch: int,
     peerLastZxid: Zxid,
     syncMode: SyncMode
@@ -56,8 +57,9 @@ predicate LearnerHandlerInit(s:LearnerHandler, my_id:nat, follower_id:nat, confi
     && s.config == config
     && s.zkdb == zkdb
     && s.state == LH_HANDSHAKE_A
-    && s.globals == globals
+    && s.globals == globals  // write access by LearnerHandler, read only access by leader
 
+    && s.queuedPackets == []
     && s.newEpoch == -1
     && s.peerLastZxid == NullZxid
     && s.syncMode == SNAP  // default to SNAP
@@ -67,7 +69,7 @@ predicate LearnerHandlerNext(s:LearnerHandler, s':LearnerHandler, ios:seq<ZKIo>)
     match s.state 
         case LH_HANDSHAKE_A => GetEpochToPropose(s, s', ios)
         case LH_HANDSHAKE_B => WaitForEpochAck(s, s', ios)
-        case LH_DECIDE_SYNC => false
+        case LH_PREP_SYNC => false
         case LH_SYNC => false
         case LH_RUNNING => LearnerHandlerStutter(s, s')
         case LH_ERROR => LearnerHandlerStutter(s, s')
@@ -113,7 +115,7 @@ predicate WaitForEpochAck(s:LearnerHandler, s':LearnerHandler, ios:seq<ZKIo>) {
     then (
         // Proceed to state sync
         && |ios| == 0   
-        && s' == s.(state := LH_DECIDE_SYNC)
+        && s' == s.(state := LH_PREP_SYNC)
     ) else (
         // Add sender to my electingFollowers set, store peerLastZxid, and continue waiting for quorum
         if |ios| == 0 then LearnerHandlerStutter(s, s')  // Case where follower has not sent anything
@@ -133,6 +135,34 @@ predicate WaitForEpochAck(s:LearnerHandler, s':LearnerHandler, ios:seq<ZKIo>) {
 }
 
 
+predicate PrepareSync(s:LearnerHandler, s':LearnerHandler, ios:seq<ZKIo>) {
+    if ! (s.zkdb.initialized && isValidZKDatabase(s.zkdb)) then |ios| == 0 && s' == s.(state := LH_ERROR)
+    else
+    var proposals := getInMemorySuffix(s.zkdb);
+    && |ios| == 0  // no I/O in this step
+    && s' == s.(state := LH_SYNC, 
+        syncMode := s'.syncMode, //syncMode to be modified accordingly
+        queuedPackets := s'.queuedPackets) //queuedPackets to be modified accordingly
+    && if |proposals| > 0 
+        then (
+            if ZxidLt(s.zkdb.maxCommittedLog, s.peerLastZxid) 
+            then    && s'.syncMode == TRUNC
+                    && |s'.queuedPackets| == 0
+            else if ZxidLt(s.peerLastZxid, s.zkdb.maxCommittedLog) 
+            then && s'.syncMode == SNAP
+                 && |s'.queuedPackets| == 0
+            else  // peerLastZxid is in the range of my proposals list
+                if s.peerLastZxid !in proposals then s' == s.(state := LH_ERROR) 
+                else
+                && s'.syncMode == DIFF
+                && s'.queuedPackets == PrepareDiffCommits(s.my_id, proposals, s.peerLastZxid)
+       ) else (
+            && s'.syncMode == DIFF
+            && |s'.queuedPackets| == 0
+       )
+}
+
+
 /*****************************************************************************************
 *                                    Helper defs                                         *
 ******************************************************************************************/ 
@@ -140,5 +170,13 @@ predicate WaitForEpochAck(s:LearnerHandler, s':LearnerHandler, ios:seq<ZKIo>) {
 predicate IsVerifiedQuorum(my_id:nat, n:int, quorum: set<nat>) {
     && my_id in quorum
     && |quorum| >= (n/2) + 1
+}
+
+function PrepareDiffCommits(leaderId:nat, proposals:seq<Zxid>, peerLastZxid:Zxid) : seq<ZKMessage> 
+    decreases proposals
+{
+    if |proposals| == 0 then []
+    else if peerLastZxid in proposals then PrepareDiffCommits(leaderId, proposals[1..], peerLastZxid)
+    else [Commit(leaderId, proposals[0])] + PrepareDiffCommits(leaderId, proposals[1..], peerLastZxid)
 }
 }
